theories/max_brute_force.v
@@ -1,8 +1,10 @@
-From Coq Require Import Floats Sint63 Uint63 QArith Lia List PArray.
+From Coq Require Import Floats Sint63 Uint63 QArith Lia List PArray Derive.
 From NeuralNetInterp.Torch Require Import Tensor Einsum Slicing.
 From NeuralNetInterp Require Import max_parameters max max_heuristics.
 From NeuralNetInterp.Util Require Import Pointed.
 From NeuralNetInterp.Util.Arith Require Import Classes Instances FloatArith.
+From NeuralNetInterp.Torch Require Import Tensor.Instances.
+From NeuralNetInterp Require Import max_instances.
 From NeuralNetInterp Require Import max_all_logits.
 Local Open Scope uint63_scope.
 Local Open Scope core_scope.
@@ -13,12 +15,28 @@ Definition totalf : float := Eval vm_compute in PrimFloat.of_uint63 total.
 Definition expected_correctf : float := Eval vm_compute in PrimFloat.of_uint63 expected_correct.
 Definition expected_accuracy : float := Eval vm_compute in expected_correctf / totalf.
 
-Time Definition computed_accuracy : float
-  := Eval vm_compute in Tensor.item (acc_fn (return_per_token := false) all_tokens_logits all_tokens).
+Definition real_accuracy : float
+  := Tensor.item (acc_fn (return_per_token := false) (logits all_tokens) all_tokens).
+
+Set NativeCompute Timing.
+
+Derive computed_accuracy SuchThat (computed_accuracy = real_accuracy) As computed_accuracy_eq.
+Proof.
+  cbv [real_accuracy].
+  etransitivity; revgoals.
+  { apply Tensor.item_Proper; intro.
+    eapply acc_fn_Proper; repeat intro; subst.
+    2-3: reflexivity.
+    apply all_tokens_logits_eq. }
+  Time vm_compute; reflexivity.
+Defined.
 
 Definition error : float := Eval cbv in (20 / totalf)%float.
 Compute abs (computed_accuracy - expected_accuracy). (*      = 0.0023193359375%float *)
 Compute (abs (computed_accuracy - expected_accuracy) * totalf)%float. (* = 19 *) (* probably from floating point assoc issues, etc *)
 Compute Qred (PrimFloat.to_Q (computed_accuracy * totalf)) / Qred (PrimFloat.to_Q totalf). (*      = 8154 # 8192 *)
-Theorem good_accuracy : (abs (computed_accuracy - expected_accuracy) <? (20 / totalf))%float = true.
-Proof. vm_compute; reflexivity. Qed.
+Theorem good_accuracy : (abs (real_accuracy - expected_accuracy) <? error)%float = true.
+Proof.
+  rewrite <- computed_accuracy_eq.
+  vm_compute; reflexivity.
+Qed.
