theories/Torch/Slicing/Instances.v
@@ -1,0 +1,137 @@
+From Coq Require Import Sint63 Uint63 Setoid Morphisms Eqdep_dec.
+From NeuralNetInterp.Torch Require Import Tensor Slicing Tensor.Instances.
+From NeuralNetInterp.Util Require Import Slice Arith.Classes Arith.Instances PolymorphicOption Nat Notations.
+From NeuralNetInterp.Util.Tactics Require Import DestructHead BreakMatch.
+Set Implicit Arguments.
+
+Definition invert_FancyIndexType {r s ri ro} (x : @FancyIndexType r s ri ro)
+  : (tensor IndexType s * (ri = 1 /\ ro = 0)) + (SliceIndexType ri ro)
+  := match x with
+     | tensor_index t => inl (t, (conj eq_refl eq_refl))
+     | normal_index s => inr s
+     end.
+
+Definition uninvert_FancyIndexType {r s ri ro} (x : (tensor IndexType s * (ri = 1 /\ ro = 0)) + (SliceIndexType ri ro)) : @FancyIndexType r s ri ro
+  := match x with
+     | inr s => normal_index s
+     | inl (t, pf)
+       => match ri, ro return ri = 1 /\ ro = 0 -> FancyIndexType s ri ro with
+          | 1, 0 => fun _ => tensor_index t
+          | 1, n => fun pf => match (ltac:(discriminate) : n = 0 -> False) (proj2 pf) with end
+          | n, _ => fun pf => match (ltac:(discriminate) : n = 1 -> False) (proj1 pf) with end
+          end pf
+     end.
+
+Lemma un_invert_FancyIndexType {r s ri ro} (x : @FancyIndexType r s ri ro) : uninvert_FancyIndexType (invert_FancyIndexType x) = x.
+Proof. destruct x; cbn; reflexivity. Qed.
+
+Lemma invert_un_FancyIndexType {r s ri ro} x : invert_FancyIndexType (@uninvert_FancyIndexType r s ri ro x) = x.
+Proof.
+  destruct x; destruct_head'_prod; destruct_head'_and; subst; cbn; reflexivity.
+Qed.
+
+Definition FancyIndexType_relation {r s ri ro} : relation (@FancyIndexType r s ri ro)
+  := fun x y
+     => match invert_FancyIndexType x, invert_FancyIndexType y with
+        | inl (x, _), inl (y, _) => Tensor.eqf x y
+        | inr x, inr y => x = y
+        | inl _, _
+        | inr _, _
+          => False
+        end.
+
+#[export] Instance FancyIndexType_relation_Reflexive {r s ri ro} : Reflexive (@FancyIndexType_relation r s ri ro).
+Proof. cbv -[tensor Tensor.eqf]; intros; destruct_head' (@FancyIndexType); reflexivity. Qed.
+#[export] Instance FancyIndexType_relation_Symmetric {r s ri ro} : Symmetric (@FancyIndexType_relation r s ri ro).
+Proof. hnf; cbv [FancyIndexType_relation]; intros; break_innermost_match; destruct_head'_prod; try assumption; symmetry; assumption. Qed.
+#[export] Instance FancyIndexType_relation_Transitive {r s ri ro} : Transitive (@FancyIndexType_relation r s ri ro).
+Proof. hnf; cbv [FancyIndexType_relation]; intros *; break_innermost_match; destruct_head'_prod; intuition auto; etransitivity; typeclasses eauto with core. Qed.
+
+Module SliceIndex.
+  Export SliceIndex.
+  Module SliceIndexType.
+    Export SliceIndexType.
+
+    #[export] Instance slice_Proper {A ris ros ri ro transfer_shape_idxs slice_idxs idx s R}
+      {slice_idxs_Proper : forall {s}, Proper (Tensor.eqfR R ==> Tensor.eqfR R) (@slice_idxs s)}
+      : Proper (Tensor.eqfR R ==> Tensor.eqfR R)
+          (@slice A ris ros ri ro transfer_shape_idxs (@slice_idxs) idx s).
+    Proof.
+      cbv [slice]; destruct idx; repeat intro; apply slice_idxs_Proper; try assumption; repeat intro; eauto.
+    Qed.
+  End SliceIndexType.
+  Export (hints) SliceIndexType.
+
+  #[export] Instance slice_Proper {A ri ro idxs s R} : Proper (Tensor.eqfR R ==> Tensor.eqfR R) (@slice A ri ro idxs s).
+  Proof.
+    induction idxs; cbn [slice]; repeat intro; eauto.
+    apply SliceIndexType.slice_Proper; eauto.
+  Qed.
+End SliceIndex.
+Export (hints) SliceIndex.
+
+Module FancyIndex.
+  Export FancyIndex.
+  Module FancyIndexType.
+    Export FancyIndexType.
+    #[export] Instance broadcast_Proper {rb sb ri ro} : Proper (FancyIndexType_relation ==> Tensor.eqf) (@broadcast rb sb ri ro).
+    Proof.
+      cbv [broadcast].
+      intros x y H idx.
+      rewrite <- (un_invert_FancyIndexType x),  <- (un_invert_FancyIndexType y).
+      cbv [FancyIndexType_relation] in H.
+      break_innermost_match_hyps; destruct_head'_prod; destruct_head'_and; subst; destruct_head'_False; cbn [uninvert_FancyIndexType].
+      all: try reflexivity.
+      apply Tensor.map_Proper; try assumption; repeat intro; reflexivity.
+    Qed.
+  End FancyIndexType.
+  Export (hints) FancyIndexType.
+
+  Inductive t_relation {rb sb} : forall {ri ro}, relation (@t rb sb ri ro) :=
+  | R_nil : t_relation nil nil
+  | R_elipsis {r} : t_relation (elipsis (r:=r)) (elipsis (r:=r))
+  | R_snoc {ris ros ri ro} : Proper (t_relation ==> FancyIndexType_relation ==> t_relation) (@snoc rb sb ris ros ri ro)
+  .
+
+  #[export] Instance t_relation_Reflexive {r s ri ro} : Reflexive (@t_relation r s ri ro).
+  Proof. intro H; induction H; constructor; auto; reflexivity. Qed.
+  #[export] Instance t_relation_Symmetric {r s ri ro} : Symmetric (@t_relation r s ri ro).
+  Proof.
+    intros x y H.
+    induction H; constructor; eauto; symmetry; assumption.
+  Qed.
+  #[export] Instance t_relation_Transitive {r s ri ro} : Transitive (@t_relation r s ri ro).
+  Proof.
+    intros x y z H1 H2.
+    induction H1; inversion H2; clear H2; inversion_sigma; subst.
+    all: cbv [Rank] in *.
+    all: repeat first [ progress cbn in *
+                      | match goal with
+                        | [ H : ?x = ?x :> nat |- _ ] => pose proof (UIP_refl_nat _ H); subst H
+                        end ].
+    all: constructor; eauto.
+    etransitivity; typeclasses eauto with core.
+  Qed.
+
+  #[export] Instance broadcast_Proper {rb sb ri ro}
+    : Proper (t_relation ==> Tensor.eqf) (@broadcast rb sb ri ro).
+  Proof.
+    intros ?? Hidxs.
+    induction Hidxs; cbn [broadcast].
+    all: try apply Tensor.map2_Proper; cbv [pointwise_relation]; intros.
+    all: eauto.
+    all: try apply FancyIndexType.broadcast_Proper.
+    all: try reflexivity.
+    all: try assumption.
+  Qed.
+
+  (* TODO: dep *)
+  #[export] Instance slice_Proper {A rb sb ri ro idxs s}
+    : Proper (Tensor.eqf ==> Tensor.eqf) (@slice A rb sb ri ro idxs s).
+  Proof.
+    cbv [slice slice_ Tensor.map_dep]; repeat intro.
+    apply Tensor.reshape_app_combine'_Proper; repeat intro.
+    apply SliceIndex.slice_Proper; assumption.
+  Qed.
+End FancyIndex.
+Export (hints) FancyIndex.
