theories/Torch/Tensor/Instances.v
@@ -4,185 +4,205 @@ From NeuralNetInterp.Util Require Nat.
 From NeuralNetInterp.Util Require Import Wf_Uint63 Wf_Uint63.Instances PArray.Proofs PArray.Instances List.Proofs Default Pointed PArray List Notations Arith.Classes Arith.Instances Bool (*PrimitiveProd*).
 From NeuralNetInterp.Torch Require Import Tensor.
 
-Definition eqfR {r A s} R : relation (@tensor r A s)
-  := pointwise_relation _ R.
-Notation eqf := (eqfR eq).
+Module Tensor.
+  Definition eqfR {r A s} R : relation (@tensor r A s)
+    := pointwise_relation _ R.
+  Notation eqf := (eqfR eq).
 
-#[export] Instance eqf_Reflexive {r A s R} {_ : Reflexive R} : Reflexive (@eqfR r A s R).
-Proof. repeat intro; subst; reflexivity. Qed.
-#[export] Instance eqf_Symmetric {r A s R} {_ : Symmetric R} : Symmetric (@eqfR r A s R).
-Proof. cbv; repeat intro; subst; symmetry; auto. Qed.
-#[export] Instance eqf_Transitive {r A s R} {_ : Transitive R} : Transitive (@eqfR r A s R).
-Proof. intros x y z H1 H2; repeat intro; subst; etransitivity; [ eapply H1 | eapply H2 ]; reflexivity. Qed.
+  #[export] Instance eqf_Reflexive {r A s R} {_ : Reflexive R} : Reflexive (@eqfR r A s R).
+  Proof. repeat intro; subst; reflexivity. Qed.
+  #[export] Instance eqf_Symmetric {r A s R} {_ : Symmetric R} : Symmetric (@eqfR r A s R).
+  Proof. cbv; repeat intro; subst; symmetry; auto. Qed.
+  #[export] Instance eqf_Transitive {r A s R} {_ : Transitive R} : Transitive (@eqfR r A s R).
+  Proof. intros x y z H1 H2; repeat intro; subst; etransitivity; [ eapply H1 | eapply H2 ]; reflexivity. Qed.
 
-Module PArray.
-  Import Tensor.PArray.
-  #[export] Instance concretize_Proper {r A default s} : Proper (eqf ==> eq) (@concretize r A default s).
-  Proof.
-    cbv [eqf Proper respectful]; revert A default s; induction r; cbn [concretize]; intros A default s t1 t2 H; auto; [].
-    destruct s.
-    eapply IHr; repeat intro; subst.
-    apply PArray.init_default_Proper; try reflexivity; repeat intro; subst.
-    apply H.
-  Qed.
+  Module PArray.
+    Import Tensor.PArray.
+    #[export] Instance concretize_Proper {r A default s} : Proper (eqf ==> eq) (@concretize r A default s).
+    Proof.
+      cbv [eqf Proper respectful]; revert A default s; induction r; cbn [concretize]; intros A default s t1 t2 H; auto; [].
+      destruct s.
+      eapply IHr; repeat intro; subst.
+      apply PArray.init_default_Proper; try reflexivity; repeat intro; subst.
+      apply H.
+    Qed.
 
-  #[export] Instance reabstract_Proper {r A s} : Proper (eqf ==> eq ==> eqf) (@reabstract r A s).
-  Proof. cbv [reabstract]; repeat intro; subst; destruct andb; eauto. Qed.
+    #[export] Instance reabstract_Proper {r A s} : Proper (pointwise_relation _ eqf ==> eq ==> eqf) (@reabstract r A s).
+    Proof. cbv [reabstract pointwise_relation eqf]; repeat intro; subst; destruct andb; eauto. Qed.
 
-  #[export] Instance checkpoint_Proper {r A default s} : Proper (eqf ==> eqf) (@checkpoint r A default s).
-  Proof. cbv [checkpoint]; repeat intro; subst; apply reabstract_Proper; try apply concretize_Proper; auto. Qed.
-End PArray.
-Export (hints) PArray.
+    #[export] Instance checkpoint_Proper {r A default s} : Proper (eqf ==> eqf) (@checkpoint r A default s).
+    Proof. cbv [checkpoint]; repeat intro; subst; apply reabstract_Proper; try apply concretize_Proper; repeat intro; auto. Qed.
+  End PArray.
+  Export (hints) PArray.
 
-Module List.
-  Import Tensor.List.
-  #[export] Instance concretize_Proper {r A s} : Proper (eqf ==> eq) (@concretize r A s).
-  Proof.
-    cbv [eqf Proper respectful]; revert A s; induction r; cbn [concretize]; intros A s t1 t2 H; auto; [].
-    destruct s.
-    eapply IHr; repeat intro; subst.
-    apply map_ext; intro.
-    apply H.
-  Qed.
+  Module List.
+    Import Tensor.List.
+    #[export] Instance concretize_Proper {r A s} : Proper (eqf ==> eq) (@concretize r A s).
+    Proof.
+      cbv [eqf Proper respectful]; revert A s; induction r; cbn [concretize]; intros A s t1 t2 H; auto; [].
+      destruct s.
+      eapply IHr; repeat intro; subst.
+      apply map_ext; intro.
+      apply H.
+    Qed.
 
-  #[export] Instance reabstract_Proper {r A default s} : Proper (eqf ==> eq ==> eqf) (@reabstract r A default s).
-  Proof. cbv [reabstract]; repeat intro; subst; match goal with |- context[match ?x with _ => _ end] => destruct x end; eauto. Qed.
+    #[export] Instance reabstract_Proper {r A default s} : Proper (pointwise_relation _ eqf ==> eq ==> eqf) (@reabstract r A default s).
+    Proof. cbv [reabstract pointwise_relation eqf]; repeat intro; subst; match goal with |- context[match ?x with _ => _ end] => destruct x end; eauto. Qed.
 
-  #[export] Instance checkpoint_Proper {r A default s} : Proper (eqf ==> eqf) (@checkpoint r A default s).
-  Proof. cbv [checkpoint]; repeat intro; subst; apply reabstract_Proper; try apply concretize_Proper; auto. Qed.
-End List.
-Export (hints) List.
+    #[export] Instance checkpoint_Proper {r A default s} : Proper (eqf ==> eqf) (@checkpoint r A default s).
+    Proof. cbv [checkpoint]; repeat intro; subst; apply reabstract_Proper; try apply concretize_Proper; repeat intro; auto. Qed.
+  End List.
+  Export (hints) List.
 
-#[export] Instance raw_get_Proper {r A s} : Proper (eqf ==> eq ==> eq) (@raw_get r A s).
-Proof. cbv -[tensor RawIndex]; intros; subst; eauto. Qed.
-#[export] Instance get_Proper {r A s} : Proper (eqf ==> eq ==> eq) (@get r A s).
-Proof. cbv -[tensor RawIndex adjust_indices_for]; intros; subst; eauto. Qed.
-#[export] Instance item_Proper {A} : Proper (eqf ==> eq) (@item A) := _.
-(*
+  #[export] Instance raw_get_Proper {r A s} : Proper (eqf ==> eq ==> eq) (@raw_get r A s).
+  Proof. cbv -[tensor RawIndex]; intros; subst; eauto. Qed.
+  #[export] Instance get_Proper {r A s} : Proper (eqf ==> eq ==> eq) (@get r A s).
+  Proof. cbv -[tensor RawIndex adjust_indices_for]; intros; subst; eauto. Qed.
+  #[export] Instance item_Proper {A} : Proper (eqf ==> eq) (@item A) := _.
+  (*
 Definition curried_raw_get {r A} {s : Shape r} (t : tensor A s) : @RawIndex.curriedT r A
   := RawIndex.curry (fun idxs => raw_get t idxs).
 Definition curried_get {r A} {s : Shape r} (t : tensor A s) : @Index.curriedT r A
   := Index.curry (fun idxs => get t idxs).
- *)
+   *)
 
-Local Ltac t_step :=
-  first [ progress subst
-        | intro
-        | reflexivity
-        | match goal with
-          | [ H : context[_ = _] |- _ ] => rewrite H
-          end
-        | solve [ eauto ]
-        | match goal with
-          | [ |- context[match ?x with _ => _ end] ] => destruct x eqn:?
-          end ].
-Local Ltac t := repeat t_step.
+  Local Ltac t_step :=
+    first [ progress subst
+          | intro
+          | reflexivity
+          | match goal with
+            | [ H : context[_ = _] |- _ ] => rewrite H
+            end
+          | solve [ eauto ]
+          | match goal with
+            | [ |- context[match ?x with _ => _ end] ] => destruct x eqn:?
+            end ].
+  Local Ltac t := repeat t_step.
 
-#[export] Instance map_Proper_R {r A B s RA RB} : Proper ((RA ==> RB) ==> eqfR RA ==> eqfR RB) (@map r A B s).
-Proof. cbv -[tensor RawIndex]; t. Qed.
-#[export] Instance map2_Proper_R {r A B C sA sB RA RB RC} : Proper ((RA ==> RB ==> RC) ==> eqfR RA ==> eqfR RB ==> eqfR RC) (@map2 r A B C sA sB).
-Proof. cbv -[tensor RawIndex]; t. Qed.
-#[export] Instance map3_Proper_R {r A B C D sA sB sC RA RB RC RD} : Proper ((RA ==> RB ==> RC ==> RD) ==> eqfR RA ==> eqfR RB ==> eqfR RC ==> eqfR RD) (@map3 r A B C D sA sB sC).
-Proof. cbv -[tensor RawIndex]; t. Qed.
+  #[export] Instance map_Proper_R {r A B s RA RB} : Proper ((RA ==> RB) ==> eqfR RA ==> eqfR RB) (@map r A B s).
+  Proof. cbv -[tensor RawIndex]; t. Qed.
+  #[export] Instance map2_Proper_R {r A B C sA sB RA RB RC} : Proper ((RA ==> RB ==> RC) ==> eqfR RA ==> eqfR RB ==> eqfR RC) (@map2 r A B C sA sB).
+  Proof. cbv -[tensor RawIndex]; t. Qed.
+  #[export] Instance map3_Proper_R {r A B C D sA sB sC RA RB RC RD} : Proper ((RA ==> RB ==> RC ==> RD) ==> eqfR RA ==> eqfR RB ==> eqfR RC ==> eqfR RD) (@map3 r A B C D sA sB sC).
+  Proof. cbv -[tensor RawIndex]; t. Qed.
 
-#[export] Instance map_Proper {r A B s RB} : Proper (pointwise_relation _ RB ==> eqf ==> eqfR RB) (@map r A B s).
-Proof. repeat intro; eapply map_Proper_R; try eassumption; repeat intro; subst; eauto. Qed.
-#[export] Instance map2_Proper {r A B C sA sB R} : Proper (pointwise_relation _ (pointwise_relation _ R) ==> eqf ==> eqf ==> eqfR R) (@map2 r A B C sA sB).
-Proof. repeat intro; eapply map2_Proper_R; try eassumption; repeat intro; subst; cbv [pointwise_relation] in *; eauto. Qed.
-#[export] Instance map3_Proper {r A B C D sA sB sC R} : Proper (pointwise_relation _ (pointwise_relation _ (pointwise_relation _ R)) ==> eqf ==> eqf ==> eqf ==> eqfR R) (@map3 r A B C D sA sB sC).
-Proof. repeat intro; eapply map3_Proper_R; try eassumption; repeat intro; subst; cbv [pointwise_relation] in *; eauto. Qed.
-(*
+  #[export] Instance map_Proper {r A B s RB} : Proper (pointwise_relation _ RB ==> eqf ==> eqfR RB) (@map r A B s).
+  Proof. repeat intro; eapply map_Proper_R; try eassumption; repeat intro; subst; eauto. Qed.
+  #[export] Instance map2_Proper {r A B C sA sB R} : Proper (pointwise_relation _ (pointwise_relation _ R) ==> eqf ==> eqf ==> eqfR R) (@map2 r A B C sA sB).
+  Proof. repeat intro; eapply map2_Proper_R; try eassumption; repeat intro; subst; cbv [pointwise_relation] in *; eauto. Qed.
+  #[export] Instance map3_Proper {r A B C D sA sB sC R} : Proper (pointwise_relation _ (pointwise_relation _ (pointwise_relation _ R)) ==> eqf ==> eqf ==> eqf ==> eqfR R) (@map3 r A B C D sA sB sC).
+  Proof. repeat intro; eapply map3_Proper_R; try eassumption; repeat intro; subst; cbv [pointwise_relation] in *; eauto. Qed.
+  (*
 Definition map_dep {r A B} {s : Shape r} (f : forall a : A, B a) (t : tensor A s) : tensor_dep B t
   := fun i => f (t i).
-*)
-#[export] Instance where__Proper {r A sA sB sC} : Proper (eqf ==> eqf ==> eqf ==> eqf) (@where_ r A sA sB sC).
-Proof. apply map3_Proper; repeat intro; reflexivity. Qed.
+   *)
+  #[export] Instance where__Proper {r A sA sB sC} : Proper (eqf ==> eqf ==> eqf ==> eqf) (@where_ r A sA sB sC).
+  Proof. apply map3_Proper; repeat intro; reflexivity. Qed.
 
-#[export] Instance tensor_add_Proper {r sA sB A B C addA RA RB RC} {_ : Proper (RA ==> RB ==> RC) addA} : Proper (eqfR RA ==> eqfR RB ==> eqfR RC) (@tensor_add r sA sB A B C addA).
-Proof. cbv [tensor_add add]; repeat intro; eapply map2_Proper_R; eassumption. Qed.
-#[export] Instance tensor_sub_Proper {r sA sB A B C subA RA RB RC} {_ : Proper (RA ==> RB ==> RC) subA} : Proper (eqfR RA ==> eqfR RB ==> eqfR RC) (@tensor_sub r sA sB A B C subA).
-Proof. cbv [tensor_sub sub]; repeat intro; eapply map2_Proper_R; eassumption. Qed.
-#[export] Instance tensor_mul_Proper {r sA sB A B C mulA RA RB RC} {_ : Proper (RA ==> RB ==> RC) mulA} : Proper (eqfR RA ==> eqfR RB ==> eqfR RC) (@tensor_mul r sA sB A B C mulA).
-Proof. cbv [tensor_mul mul]; repeat intro; eapply map2_Proper_R; eassumption. Qed.
-#[export] Instance tensor_div_by_Proper {r sA sB A B C div_byA RA RB RC} {_ : Proper (RA ==> RB ==> RC) div_byA} : Proper (eqfR RA ==> eqfR RB ==> eqfR RC) (@tensor_div_by r sA sB A B C div_byA).
-Proof. cbv [tensor_div_by div]; repeat intro; eapply map2_Proper_R; eassumption. Qed.
-#[export] Instance tensor_sqrt_Proper {r s A sqrtA R} {_ : Proper (R ==> R) sqrtA} : Proper (eqfR R ==> eqfR R) (@tensor_sqrt r s A sqrtA).
-Proof. cbv [tensor_sqrt sqrt]; repeat intro; eapply map_Proper_R; eassumption. Qed.
-#[export] Instance tensor_opp_Proper {r s A oppA R} {_ : Proper (R ==> R) oppA} : Proper (eqfR R ==> eqfR R) (@tensor_opp r s A oppA).
-Proof. cbv [tensor_opp opp]; repeat intro; eapply map_Proper_R; eassumption. Qed.
+  #[export] Instance tensor_add_Proper {r sA sB A B C addA RA RB RC} {_ : Proper (RA ==> RB ==> RC) addA} : Proper (eqfR RA ==> eqfR RB ==> eqfR RC) (@tensor_add r sA sB A B C addA).
+  Proof. cbv [tensor_add add]; repeat intro; eapply map2_Proper_R; eassumption. Qed.
+  #[export] Instance tensor_sub_Proper {r sA sB A B C subA RA RB RC} {_ : Proper (RA ==> RB ==> RC) subA} : Proper (eqfR RA ==> eqfR RB ==> eqfR RC) (@tensor_sub r sA sB A B C subA).
+  Proof. cbv [tensor_sub sub]; repeat intro; eapply map2_Proper_R; eassumption. Qed.
+  #[export] Instance tensor_mul_Proper {r sA sB A B C mulA RA RB RC} {_ : Proper (RA ==> RB ==> RC) mulA} : Proper (eqfR RA ==> eqfR RB ==> eqfR RC) (@tensor_mul r sA sB A B C mulA).
+  Proof. cbv [tensor_mul mul]; repeat intro; eapply map2_Proper_R; eassumption. Qed.
+  #[export] Instance tensor_div_by_Proper {r sA sB A B C div_byA RA RB RC} {_ : Proper (RA ==> RB ==> RC) div_byA} : Proper (eqfR RA ==> eqfR RB ==> eqfR RC) (@tensor_div_by r sA sB A B C div_byA).
+  Proof. cbv [tensor_div_by div]; repeat intro; eapply map2_Proper_R; eassumption. Qed.
+  #[export] Instance tensor_sqrt_Proper {r s A sqrtA R} {_ : Proper (R ==> R) sqrtA} : Proper (eqfR R ==> eqfR R) (@tensor_sqrt r s A sqrtA).
+  Proof. cbv [tensor_sqrt sqrt]; repeat intro; eapply map_Proper_R; eassumption. Qed.
+  #[export] Instance tensor_opp_Proper {r s A oppA R} {_ : Proper (R ==> R) oppA} : Proper (eqfR R ==> eqfR R) (@tensor_opp r s A oppA).
+  Proof. cbv [tensor_opp opp]; repeat intro; eapply map_Proper_R; eassumption. Qed.
 
 
-#[export] Instance reshape_app_split'_Proper {A r1 r2 s1 s2 R} : Proper (eqfR R ==> eqfR (eqfR R)) (@reshape_app_split' A r1 r2 s1 s2).
-Proof.
-  cbv [reshape_app_split' RawIndex.curry_radd].
-  repeat intro; eauto.
-Qed.
-#[export] Instance reshape_app_combine'_Proper {A r1 r2 s1 s2 R} : Proper (eqfR (eqfR R) ==> eqfR R) (@reshape_app_combine' A r1 r2 s1 s2).
-Proof.
-  cbv [reshape_app_combine' RawIndex.uncurry_radd].
-  repeat intro; destruct RawIndex.split_radd; cbv [eqfR pointwise_relation] in *; eauto.
-Qed.
-#[export] Instance reshape_app_split_Proper {A r1 r2 s1 s2 R} : Proper (eqfR R ==> eqfR (eqfR R)) (@reshape_app_split A r1 r2 s1 s2) := _.
-#[export] Instance reshape_app_combine_Proper {A r1 r2 s1 s2 R} : Proper (eqfR (eqfR R) ==> eqfR R) (@reshape_app_combine A r1 r2 s1 s2) := _.
-#[export] Instance reshape_snoc_split_Proper {A r s1 s2 R} : Proper (eqfR R ==> eqfR (eqfR R)) (@reshape_snoc_split A r s1 s2).
-Proof.
-  cbv [reshape_snoc_split RawIndex.curry_radd].
-  repeat intro; eauto.
-Qed.
-#[export] Instance reshape_snoc_combine_Proper {A r s1 s2 R} : Proper (eqfR (eqfR R) ==> eqfR R) (@reshape_snoc_combine A r s1 s2).
-Proof.
-  cbv [reshape_snoc_combine RawIndex.uncurry_radd].
-  repeat intro; destruct RawIndex.split_radd; cbv [eqfR pointwise_relation] in *; eauto.
-Qed.
-(*
+  #[export] Instance reshape_app_split'_Proper {A r1 r2 s1 s2 R} : Proper (eqfR R ==> eqfR (eqfR R)) (@reshape_app_split' A r1 r2 s1 s2).
+  Proof.
+    cbv [reshape_app_split' RawIndex.curry_radd].
+    repeat intro; eauto.
+  Qed.
+  #[export] Instance reshape_app_combine'_Proper {A r1 r2 s1 s2 R} : Proper (eqfR (eqfR R) ==> eqfR R) (@reshape_app_combine' A r1 r2 s1 s2).
+  Proof.
+    cbv [reshape_app_combine' RawIndex.uncurry_radd].
+    repeat intro; destruct RawIndex.split_radd; cbv [eqfR pointwise_relation] in *; eauto.
+  Qed.
+  #[export] Instance reshape_app_split_Proper {A r1 r2 s1 s2 R} : Proper (eqfR R ==> eqfR (eqfR R)) (@reshape_app_split A r1 r2 s1 s2) := _.
+  #[export] Instance reshape_app_combine_Proper {A r1 r2 s1 s2 R} : Proper (eqfR (eqfR R) ==> eqfR R) (@reshape_app_combine A r1 r2 s1 s2) := _.
+  #[export] Instance reshape_snoc_split_Proper {A r s1 s2 R} : Proper (eqfR R ==> eqfR (eqfR R)) (@reshape_snoc_split A r s1 s2).
+  Proof.
+    cbv [reshape_snoc_split RawIndex.curry_radd].
+    repeat intro; eauto.
+  Qed.
+  #[export] Instance reshape_snoc_combine_Proper {A r s1 s2 R} : Proper (eqfR (eqfR R) ==> eqfR R) (@reshape_snoc_combine A r s1 s2).
+  Proof.
+    cbv [reshape_snoc_combine RawIndex.uncurry_radd].
+    repeat intro; destruct RawIndex.split_radd; cbv [eqfR pointwise_relation] in *; eauto.
+  Qed.
+  (*
 Definition uncurry {r A} {s : Shape r} : @RawIndex.curriedT r A -> tensor A s
   := RawIndex.uncurry.
 Definition curry {r A} {s : Shape r} : tensor A s -> @RawIndex.curriedT r A
   := RawIndex.curry.
-*)
+   *)
 
-#[export] Instance map'_Proper {ra1 ra2 rb A B sa1 sa2 sb RA RB} : Proper ((eqfR RA ==> eqfR RB) ==> eqfR RA ==> eqfR RB) (@map' ra1 ra2 rb A B sa1 sa2 sb).
-Proof.
-  cbv [map']; repeat intro.
-  apply reshape_app_combine_Proper.
-  eapply map_Proper_R; try eassumption.
-  apply reshape_app_split_Proper; eassumption.
-Qed.
-#[export] Instance map2'_Proper {ri1 ri2 ro A B C sA1 sB1 sA2 sB2 so RA RB RC} : Proper ((eqfR RA ==> eqfR RB ==> eqfR RC) ==> eqfR RA ==> eqfR RB ==> eqfR RC) (@map2' ri1 ri2 ro A B C sA1 sB1 sA2 sB2 so).
-Proof.
-  cbv [map2']; repeat intro.
-  apply reshape_app_combine_Proper.
-  eapply map2_Proper_R; try eassumption.
-  all: apply reshape_app_split_Proper; eassumption.
-Qed.
+  #[export] Instance map'_Proper {ra1 ra2 rb A B sa1 sa2 sb RA RB} : Proper ((eqfR RA ==> eqfR RB) ==> eqfR RA ==> eqfR RB) (@map' ra1 ra2 rb A B sa1 sa2 sb).
+  Proof.
+    cbv [map']; repeat intro.
+    apply reshape_app_combine_Proper.
+    eapply map_Proper_R; try eassumption.
+    apply reshape_app_split_Proper; eassumption.
+  Qed.
+  #[export] Instance map2'_Proper {ri1 ri2 ro A B C sA1 sB1 sA2 sB2 so RA RB RC} : Proper ((eqfR RA ==> eqfR RB ==> eqfR RC) ==> eqfR RA ==> eqfR RB ==> eqfR RC) (@map2' ri1 ri2 ro A B C sA1 sB1 sA2 sB2 so).
+  Proof.
+    cbv [map2']; repeat intro.
+    apply reshape_app_combine_Proper.
+    eapply map2_Proper_R; try eassumption.
+    all: apply reshape_app_split_Proper; eassumption.
+  Qed.
 
-#[export] Instance broadcast_Proper {r A s R} : Proper (eqfR R ==> forall_relation (fun r' => eqfR R)) (@broadcast r A s).
-Proof.
-  cbv [broadcast broadcast' repeat']; intros ??? ?.
-  apply reshape_app_combine_Proper.
-  intro; assumption.
-Qed.
-#[export] Instance repeat_Proper {r A s R} : Proper (eqfR R ==> forall_relation (fun r' => forall_relation (fun s' => eqfR R))) (@repeat r A s).
-Proof.
-  cbv [repeat repeat']; intros ??? ? ?.
-  apply reshape_app_combine_Proper.
-  intro; assumption.
-Qed.
+  #[export] Instance broadcast_Proper {r A s R} : Proper (eqfR R ==> forall_relation (fun r' => eqfR R)) (@broadcast r A s).
+  Proof.
+    cbv [broadcast broadcast' repeat']; intros ??? ?.
+    apply reshape_app_combine_Proper.
+    intro; assumption.
+  Qed.
+  #[export] Instance repeat_Proper {r A s R} : Proper (eqfR R ==> forall_relation (fun r' => forall_relation (fun s' => eqfR R))) (@repeat r A s).
+  Proof.
+    cbv [repeat repeat']; intros ??? ? ?.
+    apply reshape_app_combine_Proper.
+    intro; assumption.
+  Qed.
 
-#[export] Instance keepdim_gen_Proper {r s A B R} : Proper (pointwise_relation _ (eqfR R) ==> eq ==> eqfR R) (@keepdim_gen r s A B).
-Proof.
-  cbv [keepdim_gen]; intros ?? H ???; subst.
-  apply broadcast_Proper; apply H.
-Qed.
-#[export] Instance keepdim_Proper {A B R} : Proper (pointwise_relation _ R ==> eq ==> eqfR R) (@keepdim A B).
-Proof.
-  cbv [keepdim]; intros ?? H ??? ?; subst; eapply keepdim_gen_Proper; t.
-Qed.
+  #[export] Instance keepdim_gen_Proper {r s A B R} : Proper (pointwise_relation _ (eqfR R) ==> eq ==> eqfR R) (@keepdim_gen r s A B).
+  Proof.
+    cbv [keepdim_gen]; intros ?? H ???; subst.
+    apply broadcast_Proper; apply H.
+  Qed.
+  #[export] Instance keepdim_Proper {A B R} : Proper (pointwise_relation _ R ==> eq ==> eqfR R) (@keepdim A B).
+  Proof.
+    cbv [keepdim]; intros ?? H ??? ?; subst; eapply keepdim_gen_Proper; t.
+  Qed.
 
-#[export] Instance reduce_axis_m1'_Proper {r A B s1 s2 RA RB} : Proper (pointwise_relation _ (pointwise_relation _ (pointwise_relation _ (pointwise_relation _ RA ==> RB))) ==> eqfR RA ==> eqfR RB) (@reduce_axis_m1' r A B s1 s2).
+  #[export] Instance reduce_axis_m1'_Proper {r A B s1 s2 RA RB} : Proper (pointwise_relation _ (pointwise_relation _ (pointwise_relation _ (pointwise_relation _ RA ==> RB))) ==> eqfR RA ==> eqfR RB) (@reduce_axis_m1' r A B s1 s2).
+  Proof.
+    cbv [reduce_axis_m1'].
+    intros ?? H ?? Ht.
+    eapply map_Proper_R; try eapply reshape_snoc_split_Proper; try eassumption.
+    intros ?? Ht'.
+    cbv [pointwise_relation eqfR respectful] in *.
+    eauto.
+  Qed.
+
+  #[export] Instance reduce_axis_m1_Proper {r A B s1 s2 keepdim RA RB}
+    : Proper (pointwise_relation _ (pointwise_relation _ (pointwise_relation _ (pointwise_relation _ RA ==> RB))) ==> eqfR RA ==> eqfR RB)
+        (@reduce_axis_m1 r A B s1 s2 keepdim).
+  Proof.
+    cbv [reduce_axis_m1]; destruct keepdim; intros ?? H ?? Ht ?.
+    all: eapply reduce_axis_m1'_Proper; try eassumption.
+  Qed.
+
+
+  (*#[export] Instance reduce_axis_m1'_Proper' {r A B s1 s2 reduction RA} : Proper (eqfR RA ==> eqf) (@reduce_axis_m1' r A B s1 s2 reduction).
 Proof.
   cbv [reduce_axis_m1'].
-  intros ?? H ?? Ht.
+  intros ?? Ht.
   eapply map_Proper_R; try eapply reshape_snoc_split_Proper; try eassumption.
   intros ?? Ht'.
   cbv [pointwise_relation eqfR respectful] in *.
@@ -197,109 +217,92 @@ Proof.
   all: eapply reduce_axis_m1'_Proper; try eassumption.
 Qed.
 
+   *)
+  #[export] Instance softmax_dim_m1_Proper {r A B C addB expA zeroB divB s0 s'}
+    : Proper (eqf ==> eqf) (@softmax_dim_m1 r A B C addB expA zeroB divB s0 s').
+  Proof.
+    intros ?? Ht.
+    cbv [softmax_dim_m1 div].
+    eapply tensor_div_by_Proper.
+    all: try eapply (@reduce_axis_m1_Proper r B B s0 s' true).
+    all: try (eapply map_Proper; try eassumption; repeat intro).
+    all: try eapply Reduction.sum_Proper_pointwise.
+    all: try exact eq_refl.
+    Unshelve.
+    repeat intro; subst; reflexivity.
+  Qed.
 
-(*#[export] Instance reduce_axis_m1'_Proper' {r A B s1 s2 reduction RA} : Proper (eqfR RA ==> eqf) (@reduce_axis_m1' r A B s1 s2 reduction).
-Proof.
-  cbv [reduce_axis_m1'].
-  intros ?? Ht.
-  eapply map_Proper_R; try eapply reshape_snoc_split_Proper; try eassumption.
-  intros ?? Ht'.
-  cbv [pointwise_relation eqfR respectful] in *.
-  eauto.
-Qed.
+  #[export] Instance log_softmax_dim_m1_Proper {r A B C D addB lnA expA zeroB divB s0 s'}
+    : Proper (eqf ==> eqf) (@log_softmax_dim_m1 r A B C D addB lnA expA zeroB divB s0 s').
+  Proof.
+    intros ?? Ht.
+    cbv [log_softmax_dim_m1 div].
+    eapply tensor_div_by_Proper; try eassumption.
+    eapply map_Proper; try eassumption.
+    all: try eapply (@reduce_axis_m1_Proper r B B s0 s' true).
+    all: try (eapply map_Proper; try eassumption; repeat intro).
+    all: try eapply Reduction.sum_Proper_pointwise.
+    all: try (repeat intro; exact eq_refl).
+    Unshelve.
+    repeat intro; subst; reflexivity.
+  Qed.
 
-#[export] Instance reduce_axis_m1_Proper {r A B s1 s2 keepdim RA RB}
-  : Proper (pointwise_relation _ (pointwise_relation _ (pointwise_relation _ (pointwise_relation _ RA ==> RB))) ==> eqfR RA ==> eqfR RB)
-      (@reduce_axis_m1 r A B s1 s2 keepdim).
-Proof.
-  cbv [reduce_axis_m1]; destruct keepdim; intros ?? H ?? Ht ?.
-  all: eapply reduce_axis_m1'_Proper; try eassumption.
-Qed.
+  #[export] Instance unsqueeze_dim_m1_Proper {A r s R} : Proper (eqfR R ==> eqfR R) (@unsqueeze_dim_m1 A r s).
+  Proof. intros ?? H; cbv; intros; apply H. Qed.
 
-*)
-#[export] Instance softmax_dim_m1_Proper {r A B C addB expA zeroB divB s0 s'}
-  : Proper (eqf ==> eqf) (@softmax_dim_m1 r A B C addB expA zeroB divB s0 s').
-Proof.
-  intros ?? Ht.
-  cbv [softmax_dim_m1 div].
-  eapply tensor_div_by_Proper.
-  all: try eapply (@reduce_axis_m1_Proper r B B s0 s' true).
-  all: try (eapply map_Proper; try eassumption; repeat intro).
-  all: try eapply sum_Proper_pointwise.
-  all: try exact eq_refl.
-  Unshelve.
-  repeat intro; subst; reflexivity.
-Qed.
+  #[export] Instance gather_dim_m1_Proper {A r ssinput ssindex sinput' sindex' R} : Proper (eqfR R ==> eqf ==> eqfR R) (@gather_dim_m1 A r ssinput ssindex sinput' sindex').
+  Proof.
+    intros ?? H1 ?? H2; cbv [gather_dim_m1]; intro.
+    rewrite H2.
+    apply H1.
+  Qed.
 
-#[export] Instance log_softmax_dim_m1_Proper {r A B C D addB lnA expA zeroB divB s0 s'}
-  : Proper (eqf ==> eqf) (@log_softmax_dim_m1 r A B C D addB lnA expA zeroB divB s0 s').
-Proof.
-  intros ?? Ht.
-  cbv [log_softmax_dim_m1 div].
-  eapply tensor_div_by_Proper; try eassumption.
-  eapply map_Proper; try eassumption.
-  all: try eapply (@reduce_axis_m1_Proper r B B s0 s' true).
-  all: try (eapply map_Proper; try eassumption; repeat intro).
-  all: try eapply sum_Proper_pointwise.
-  all: try (repeat intro; exact eq_refl).
-  Unshelve.
-  repeat intro; subst; reflexivity.
-Qed.
+  #[export] Instance squeeze_Proper {A r s R} : Proper (eqfR R ==> eqfR R) (@squeeze A r s).
+  Proof. intros ?? H; cbv; intros; apply H. Qed.
+  #[export] Instance reshape_m1_Proper {A r s R} : Proper (eqfR R ==> eqfR R) (@reshape_m1 A r s).
+  Proof. intros ?? H ?; cbv [reshape_m1]; apply H. Qed.
+  #[export] Instance unreshape_m1_Proper {A r s R} : Proper (eqfR R ==> eqfR R) (@unreshape_m1 A r s).
+  Proof. intros ?? H ?; cbv [unreshape_m1]; apply H. Qed.
 
-#[export] Instance unsqueeze_dim_m1_Proper {A r s R} : Proper (eqfR R ==> eqfR R) (@unsqueeze_dim_m1 A r s).
-Proof. intros ?? H; cbv; intros; apply H. Qed.
+  #[export] Instance to_bool_Proper {A zero eqb r s} : Proper (eqf ==> eqf) (@to_bool A zero eqb r s).
+  Proof.
+    intros ?? H ?; cbv [to_bool]; apply map_Proper; try assumption; repeat intro; reflexivity.
+  Qed.
 
-#[export] Instance gather_dim_m1_Proper {A r ssinput ssindex sinput' sindex' R} : Proper (eqfR R ==> eqf ==> eqfR R) (@gather_dim_m1 A r ssinput ssindex sinput' sindex').
-Proof.
-  intros ?? H1 ?? H2; cbv [gather_dim_m1]; intro.
-  rewrite H2.
-  apply H1.
-Qed.
-
-#[export] Instance squeeze_Proper {A r s R} : Proper (eqfR R ==> eqfR R) (@squeeze A r s).
-Proof. intros ?? H; cbv; intros; apply H. Qed.
-#[export] Instance reshape_m1_Proper {A r s R} : Proper (eqfR R ==> eqfR R) (@reshape_m1 A r s).
-Proof. intros ?? H ?; cbv [reshape_m1]; apply H. Qed.
-#[export] Instance unreshape_m1_Proper {A r s R} : Proper (eqfR R ==> eqfR R) (@unreshape_m1 A r s).
-Proof. intros ?? H ?; cbv [unreshape_m1]; apply H. Qed.
-
-#[export] Instance to_bool_Proper {A zero eqb r s} : Proper (eqf ==> eqf) (@to_bool A zero eqb r s).
-Proof.
-  intros ?? H ?; cbv [to_bool]; apply map_Proper; try assumption; repeat intro; reflexivity.
-Qed.
-
-#[export] Instance of_bool_Proper {A zero one r s} : Proper (eqf ==> eqf) (@of_bool A zero one r s).
-Proof.
-  intros ?? H ?; cbv [of_bool]; apply map_Proper; try assumption; repeat intro; reflexivity.
-Qed.
+  #[export] Instance of_bool_Proper {A zero one r s} : Proper (eqf ==> eqf) (@of_bool A zero one r s).
+  Proof.
+    intros ?? H ?; cbv [of_bool]; apply map_Proper; try assumption; repeat intro; reflexivity.
+  Qed.
 
 
-#[export] Instance mean_Proper {r A s B C zero addA div_boyABC coerB} : Proper (eqf ==> eqf) (@mean r A s B C zero addA div_boyABC coerB).
-Proof.
-  cbv [mean]; intros ?? H ?.
-  eapply reduce_axis_m1_Proper.
-  1: eapply mean_Proper_pointwise.
-  apply reshape_m1_Proper.
-  assumption.
-Qed.
+  #[export] Instance mean_Proper {r A s B C zero addA div_boyABC coerB} : Proper (eqf ==> eqf) (@mean r A s B C zero addA div_boyABC coerB).
+  Proof.
+    cbv [mean]; intros ?? H ?.
+    eapply reduce_axis_m1_Proper.
+    1: eapply Reduction.mean_Proper_pointwise.
+    apply reshape_m1_Proper.
+    assumption.
+  Qed.
 
-(*(* TODO: nary *)
+  (*(* TODO: nary *)
 Definition tupleify {A B s1 s2} (t1 : tensor A [s1]) (t2 : tensor B [s2]) : tensor (A * B) [s1; s2]
   := fun '((tt, a), b) => (raw_get t1 [a], raw_get t2 [b]).
 Definition cartesian_prod {A s1 s2} (t1 : tensor A [s1]) (t2 : tensor A [s2]) : tensor A [s1 * s2; 2]
   := fun '((tt, idx), tuple_idx)
      => let '(a, b) := raw_get (reshape_m1 (tupleify t1 t2)) [idx] in
         nth_default a [a; b] (Z.to_nat (Uint63.to_Z (tuple_idx mod 2))).
- *)
-#[export] Instance tril_Proper {A zeroA rnk s r c diagonal} : Proper (eqf ==> eqf) (@tril A zeroA rnk s r c diagonal).
-Proof.
-  cbv [tril]; intros ?? H [[? ?] ?].
-  rewrite H.
-  reflexivity.
-Qed.
-#[export] Instance triu_Proper {A zeroA rnk s r c diagonal} : Proper (eqf ==> eqf) (@triu A zeroA rnk s r c diagonal).
-Proof.
-  cbv [triu]; intros ?? H [[? ?] ?].
-  rewrite H.
-  reflexivity.
-Qed.
+   *)
+  #[export] Instance tril_Proper {A zeroA rnk s r c diagonal} : Proper (eqf ==> eqf) (@tril A zeroA rnk s r c diagonal).
+  Proof.
+    cbv [tril]; intros ?? H [[? ?] ?].
+    rewrite H.
+    reflexivity.
+  Qed.
+  #[export] Instance triu_Proper {A zeroA rnk s r c diagonal} : Proper (eqf ==> eqf) (@triu A zeroA rnk s r c diagonal).
+  Proof.
+    cbv [triu]; intros ?? H [[? ?] ?].
+    rewrite H.
+    reflexivity.
+  Qed.
+End Tensor.
+Export (hints) Tensor.
